generate redesigned semantics theories

isa/Gencot_CArray_Tuples.thy
@@ -4,114 +4,173 @@ theory Gencot_CArray_Tuples
   "HOL-Library.Adhoc_Overloading"
 begin
 
-text \<open>Declare pointer referencing / dereferencing functions for modrefArr.
-These must be overloaded for every type which occurs as element type of an array.\<close>
+section \<open>Gencot Array Operations\<close>
+
+text \<open>
+Gencot array operations are polymorphic on the type of the array elements, the size of the array and
+on the type of the index values. 
+
+Gencot array types are represented by HOL lists in Isabelle. For every Gencot array type a conversion
+to and from lists is defined. These conversion functions are polymorphic on the element type and the
+array size. Then every abstract Gencot array operations is defined by
+the conversion functions together with a usual operation on lists, which is only polymorphic on the
+list element type but not on the list size. The list size restrictions are covered by defining an 
+additional function for specifying the array size, polymorphic on the element type. The actual 
+restrictions are not specified here, since they are not needed for the refinement proof.
+
+The index values are always assumed to be values of type \<open>'m word\<close> for some bitlength \<open>'m\<close>. So
+the polymorphism is reduced on the bitlength \<open>'m\<close>. For actual programs only the bitlengths \<open>8\<close>,
+\<open>16\<close>, \<open>32\<close>, and \<open>64\<close> are used, corresponding to the Cogent types U8, U16, U32, U64 used for indexes.
+
+Here the Gencot array types are called ``carrays'' and the restricted lists are called ``arrays''.
+The carrays are denoted by the type variable \<open>'carr\<close>.
+\<close>
+
+subsection \<open>Global Names for Polymorphic Functions\<close>
+
+text \<open>
+Polymorphic functions are specified by overloading a global name. If definitions or laws 
+shall be available for them, corresponding attributes are defined for collecting them in buckets.
+
+The conversion functions are \<open>arr\<close> for conversion
+from carray to array and \<open>carr\<close> for the opposite conversion. The size function is \<open>siz\<close>.
+Attributes are introduced for collecting the definitions of the conversion functions and the 
+size function.
+\<close>
+
+consts
+  arr :: "'carr \<Rightarrow> 'el list"
+  carr :: "'el list \<Rightarrow> 'carr"
+  siz :: "'carr \<Rightarrow> nat"
+
+ML \<open>structure arr_def = Named_Thms (val name = Binding.name "arr_def" val description = "")\<close>
+setup \<open> arr_def.setup \<close>
+ML \<open>structure carr_def = Named_Thms (val name = Binding.name "carr_def" val description = "")\<close>
+setup \<open> carr_def.setup \<close>
+ML \<open>structure siz_def = Named_Thms (val name = Binding.name "siz_def" val description = "")\<close>
+setup \<open> siz_def.setup \<close>
+
+text \<open>
+For the Gencot array operations the global names are declared by the Cogent compiler when it
+translates their abstract Cogent declarations. No attributes are introduced for their definitions.
+\<close>
+
+text \<open>
+For the definition of \<open>modrefArr\<close> pointer referencing / dereferencing functions for the array
+elements are required.
+These must be overloaded for every type which occurs as element type of an array in a Cogent program.
+\<close>
 
 consts
   toPtr :: "'el \<Rightarrow> 'pel"
   frPtr :: "'pel \<Rightarrow> 'el"
 
-text \<open>Define the array functions for fixed lists\<close>
+subsection \<open>Definitions for the Gencot Array Operations\<close>
 
-definition getArr' :: "('n::len, 'el) FixedList \<Rightarrow> 'idx::len word \<Rightarrow> 'el"
-  where 
-    "getArr' lst idx \<equiv>
-      if unat idx >= LENGTH('n) then hd (Rep_FixedList lst)
-      else (nth (Rep_FixedList lst) (unat idx))"
+text \<open>
+The definitions of the polymorphic array operations are specified in a locale. For every 
+Gencot array type the operation instances are defined by interpreting the locale. The locale
+parameters are the conversion and size functions. The bitlength \<open>'m\<close> of the index type is specified 
+by an arbitrary constant of type \<open>'m word\<close>, usually the value \<open>0\<close> can be used for it.\<close>
 
-definition setArr' :: "('n::len, 'el) FixedList \<Rightarrow> 'idx::len word \<Rightarrow> 'el \<Rightarrow> ('n, 'el) FixedList"
-  where
-    "setArr' lst idx elm \<equiv> 
-      if unat idx >= LENGTH('n) then lst
-      else (Abs_FixedList (list_update (Rep_FixedList lst) (unat idx) elm))"
-
-definition modifyArr' :: "('n::len, 'el) FixedList \<Rightarrow> 'idx::len word \<Rightarrow> ('el \<times> 'arg \<Rightarrow> 'el \<times> 'out) \<Rightarrow> 'arg \<Rightarrow> ('n, 'el) FixedList \<times> 'out"
-  where
-    "modifyArr' lst idx chf inp \<equiv> 
-      let i = (if unat idx >= LENGTH('n) then 0 else unat idx); 
-          l = Rep_FixedList lst; elm = nth l i; chres = chf(elm, inp)
-      in (Abs_FixedList (list_update l i (fst chres)), snd chres)"
-
-definition modrefArr' :: "('n::len, 'el) FixedList \<Rightarrow> 'idx::len word \<Rightarrow> ('pel \<times> 'arg \<Rightarrow> 'pel \<times> 'out) \<Rightarrow> 'arg \<Rightarrow> ('n, 'el) FixedList \<times> 'out"
-  where
-    "modrefArr' lst idx chf inp \<equiv> 
-      let i = (if unat idx >= LENGTH('n) then 0 else unat idx); 
-          l = Rep_FixedList lst; elm = nth l i; chres = chf(toPtr elm, inp)
-      in (Abs_FixedList (list_update l i (frPtr (fst chres))), snd chres)"
-
-definition toCAES' :: "('n::len, 'el) FixedList \<Rightarrow> 'el CArrES\<^sub>T"
-  where "toCAES' lst \<equiv> (Rep_FixedList lst, of_nat LENGTH('n))"
-
-definition fromCAES' :: "'el CArrES\<^sub>T \<Rightarrow> ('n::len, 'el) FixedList"
-  where "fromCAES' aes \<equiv> Abs_FixedList (fst aes) "
-
-text \<open>For every actual wrapper record the following locale will be interpreted.
-      It takes the wrapper record access and constructor as parameters.
-      The locale defines specific array functions for the wrapper record.\<close>
-
-locale CArrFuns = 
-  fixes 
-    fld :: "'arr \<Rightarrow> ('n::len, 'el) FixedList" and 
-    wrp :: "('n, 'el) FixedList \<Rightarrow> 'arr"
+locale GencotArrDefs = 
+  fixes arr :: "'carr \<Rightarrow> 'el list"
+    and carr :: "'el list \<Rightarrow> 'carr"
+    and siz :: "'carr \<Rightarrow> nat"
+    and idxtypespec :: "('m::len) word"
 begin
-text \<open>Lift the array functions from fixed lists to the wrapper record.\<close>
-definition getArrFxd :: "'arr \<times> ('m::len) word \<Rightarrow> 'el"
-  where "getArrFxd arg \<equiv> let (arr,idx) = arg in getArr' (fld arr) idx"
-definition setArrFxd :: "'arr \<times> ('m::len) word \<times> 'el \<Rightarrow> 'arr \<times> unit"
-  where "setArrFxd arg \<equiv> let (arr,idx,elm) = arg in (wrp(setArr' (fld arr) idx elm), ())"
-definition modifyArrFxd :: "'arr \<times> ('m::len) word \<times> ('el \<times> 'arg \<Rightarrow> 'el \<times> 'out) \<times> 'arg \<Rightarrow> 'arr \<times> 'out"
-  where "modifyArrFxd arg \<equiv> let (arr, idx, chf, inp) = arg; 
-    (reslst,res) = modifyArr' (fld arr) idx chf inp in (wrp reslst, res)"
-definition modrefArrFxd :: "'arr \<times> ('m::len) word \<times> ('pel \<times> 'arg \<Rightarrow> 'pel \<times> 'out) \<times> 'arg \<Rightarrow> 'arr \<times> 'out"
-  where "modrefArrFxd arg \<equiv> let (arr, idx, chf, inp) = arg; 
-    (reslst,res) = modrefArr' (fld arr) idx chf inp in (wrp reslst, res)"
+definition getArr :: "'carr \<times> 'm word \<Rightarrow> 'el"
+  where "getArr arg \<equiv> let (c,i) = arg in 
+            if unat i \<ge> siz c then hd (arr c) else (nth (arr c) (unat i))"
+definition setArr :: "'carr \<times> 'm word \<times> 'el \<Rightarrow> 'carr \<times> unit"
+  where "setArr arg \<equiv> let (c,i,e) = arg in 
+            (if unat i \<ge> siz c then c else carr (list_update (arr c) (unat i) e), ())"
+definition modifyArr :: "'carr \<times> 'm word \<times> ('el \<times> 'arg \<Rightarrow> 'el \<times> 'out) \<times> 'arg \<Rightarrow> 'carr \<times> 'out"
+  where "modifyArr arg \<equiv> 
+    let (c, idx, u, inp) = arg;
+        i = (if unat idx \<ge> siz c then 0 else unat idx);
+        ures = u(nth (arr c) i, inp) 
+    in (carr (list_update (arr c) i (fst ures)), snd ures)"
+definition modrefArr :: "'carr \<times> 'm word \<times> ('pel \<times> 'arg \<Rightarrow> 'pel \<times> 'out) \<times> 'arg \<Rightarrow> 'carr \<times> 'out"
+  where "modrefArr arg \<equiv> 
+    let (c, idx, u, inp) = arg; 
+        i = (if unat idx \<ge> siz c then 0 else unat idx); 
+        ures = u(toPtr (nth (arr c) i), inp)
+    in (carr (list_update (arr c) i (frPtr (fst ures))), snd ures)"
+end
 
-definition toCAESFxd :: "'arr \<Rightarrow> 'el CArrES\<^sub>T"
-  where "toCAESFxd arr \<equiv> toCAES' (fld arr)"
-definition fromCAESFxd :: "'el CArrES\<^sub>T \<Rightarrow> 'arr"
-  where "fromCAESFxd aes \<equiv> wrp (fromCAES' aes)"
-definition rotoCAESFxd :: "'arr \<Rightarrow> 'el CArrES\<^sub>T"
-  where "rotoCAESFxd arr \<equiv> toCAES' (fld arr)"
-definition rofromCAESFxd :: "'el CArrES\<^sub>T \<Rightarrow> 'arr"
-  where "rofromCAESFxd aes \<equiv> wrp (fromCAES' aes)"
+subsection \<open>Explicitly sized arrays\<close>
+
+text \<open>
+An explicitly sized array is a pair consisting of a list and the explicitly specified size as a 64 bit word.
+Indexes always have bitlength \<open>64\<close>.
+\<close>
+
+definition arrES :: "'el CArrES\<^sub>T \<Rightarrow> 'el list" 
+  where [arr_def]: "arrES \<equiv> fst"
+definition carrES :: "'el list \<Rightarrow> 'el CArrES\<^sub>T" 
+  where [carr_def]: "carrES \<equiv> \<lambda>a. (a,of_nat (length a))"
+definition sizES :: "'el CArrES\<^sub>T \<Rightarrow> nat" 
+  where [siz_def]: "sizES \<equiv> (unat \<circ> snd)"
+
+interpretation ESArrDefs: GencotArrDefs arrES carrES sizES "0::64 word" .
+adhoc_overloading 
+      arr arrES
+  and carr carrES
+  and siz sizES
+  and getArr ESArrDefs.getArr
+  and setArr ESArrDefs.setArr
+  and modifyArr ESArrDefs.modifyArr
+  and modrefArr ESArrDefs.modrefArr
+
+subsection \<open>Fixed sized arrays\<close>
+
+text \<open>
+For fixed sized arrays there is a type for every size used in the Cogent program.
+In addition to the normal Gencot array operations Gencot defines polymorphic conversion
+functions from and to explicitly sized arrays. The following locale takes the size value
+as parameter instead of the size function. It defines the size function
+and specifies definitions for the conversion functions from/to explicitly sized arrays. 
+\<close>
+
+locale FxdArrBase = 
+  fixes arr :: "'carr \<Rightarrow> 'el list"
+    and carr :: "'el list \<Rightarrow> 'carr"
+    and fxdsiz :: "nat"
+begin
+
+definition siz :: "'carr \<Rightarrow> nat"
+  where fxdsiz_def[siz_def]: "siz c \<equiv> fxdsiz"
+
+definition toCAES :: "'carr \<Rightarrow> 'el CArrES\<^sub>T"
+  where "toCAES a \<equiv> (arr a, of_nat (fxdsiz))"
+definition fromCAES :: "'el CArrES\<^sub>T \<Rightarrow> 'carr"
+  where "fromCAES aes \<equiv> carr (arrES aes)"
+definition rotoCAES :: "'carr \<Rightarrow> 'el CArrES\<^sub>T"
+  where [simp]: "rotoCAES a \<equiv> toCAES a"
+definition rofromCAES :: "'el CArrES\<^sub>T \<Rightarrow> 'carr"
+  where [simp]: "rofromCAES aes \<equiv> fromCAES aes"
 
 end
 
-text \<open>Define the array functions for explicitly sized arrays\<close>
+text \<open>
+The following locale extends \<open>FxdArrBase\<close> and provides 
+the definitions of the normal Gencot array operations by interpreting \<open>GencotArrDefs\<close>.
 
-definition getArrES :: "'el CArrES\<^sub>T \<times> 'idx::len word \<Rightarrow> 'el"
-  where 
-    "getArrES arg \<equiv>
-      let ((lst,len),idx) = arg
-      in if unat idx >= unat len then hd lst
-         else (nth lst (unat idx))"
+It is intended to be interpreted once for every size of fixed carrays occurring in the C program,
+together with a specification for the bitlength of the index values. These interpretations only 
+provide the definitions of the Gencot array operations which is sufficient for the refinement
+proof.
+\<close>
 
-definition setArrES :: "'el CArrES\<^sub>T \<times> 'idx::len word \<times> 'el \<Rightarrow> 'el CArrES\<^sub>T \<times> unit"
-  where
-    "setArrES arg \<equiv> 
-      let ((lst,len),idx,elm) = arg
-      in if unat idx >= unat len then ((lst,len),())
-         else (((list_update lst (unat idx) elm),len),())"
-
-definition modifyArrES :: "'el CArrES\<^sub>T \<times> ('idx::len word \<times> ('el \<times> 'arg \<Rightarrow> 'el \<times> 'out) \<times> 'arg) \<Rightarrow> 'el CArrES\<^sub>T \<times> 'out"
-  where
-    "modifyArrES arg \<equiv> 
-      let ((lst,len),(idx,chf,inp)) = arg;
-          i = (if unat idx < unat len then (unat idx) else 0);
-          elm = nth lst i; chres = chf(elm, inp)
-      in ((list_update lst i (fst chres),len), snd chres)"
-
-definition modrefArrES :: "'el CArrES\<^sub>T \<times> ('idx::len word \<times> ('pel \<times> 'arg \<Rightarrow> 'pel \<times> 'out) \<times> 'arg) \<Rightarrow> 'el CArrES\<^sub>T \<times> 'out"
-  where
-    "modrefArrES arg \<equiv> 
-      let ((lst,len),(idx,chf,inp)) = arg;
-          i = (if unat idx < unat len then (unat idx) else 0);
-          elm = nth lst i; chres = chf(toPtr elm, inp)
-      in ((list_update lst i (frPtr (fst chres)),len), snd chres)"
-
-adhoc_overloading getArr getArrES
-  and setArr setArrES
-  and modifyArr modifyArrES
-  and modrefArr modrefArrES
+locale FxdArrDefs = FxdArrBase arr carr fxdsiz
+  for arr :: "'carr \<Rightarrow> 'el list"
+  and carr :: "'el list \<Rightarrow> 'carr"
+  and fxdsiz :: "nat"
++ 
+fixes idxtypespec :: "('m::len) word"
+begin
+sublocale GencotArrDefs arr carr siz idxtypespec .
+end
 
 end
