isa/Gencot_SemanticsSupport.thy
@@ -1,0 +1,10 @@
+theory Gencot_SemanticsSupport
+  imports 
+    Gencot_PartAccessSupport
+    Gencot_ArraySupport
+begin
+ML \<open>structure sem = Named_Thms (val name = Binding.name "sem" val description = "")\<close>
+setup \<open> sem.setup \<close>
+ML \<open>structure sem_defs = Named_Thms (val name = Binding.name "sem_defs" val description = "")\<close>
+setup \<open> sem_defs.setup \<close>
+end
